Updated competition with harmonic oscilator.

ARCH2022_Examples.thy
@@ -7,6 +7,7 @@ theory ARCH2022_Examples
   imports 
     HS_Lie_Derivatives
     Real_Arith_Tactics
+    "Matrices/MTX_Flows"
 
 begin
 
@@ -2640,6 +2641,222 @@ lemma "`em = 0 \<and> d \<ge> 0 \<and> b > 0 \<and> \<epsilon> > 0 \<and> A > 0 
    apply (safe; clarsimp simp: dlo_simps)
       apply (metis diff_zero)
   oops
+
+end
+
+lemma overdamped_door_arith:
+  assumes "b\<^sup>2 + 4 * a > 0" and "a < 0" and "b \<le> 0" and "t \<ge> 0" and "k > 0"
+  shows "k * (b - sqrt (b\<^sup>2 + 4 * a)) * exp (t * (b + sqrt (b\<^sup>2 + 4 * a)) / 2) / (2 * sqrt (b\<^sup>2 + 4 * a))
+       \<le> k * (b + sqrt (b\<^sup>2 + 4 * a)) * exp (t * (b - sqrt (b\<^sup>2 + 4 * a)) / 2) / (2 * sqrt (b\<^sup>2 + 4 * a))"
+proof-
+  have f0: "k / (2 * sqrt (b\<^sup>2 + a * 4)) \<ge> 0"  (is "k/?c3 \<ge> 0")
+    using assms(1,5) by simp
+  have f1: "(b - sqrt (b\<^sup>2 + 4 * a)) < (b + sqrt (b\<^sup>2 + 4 * a))" (is "?c2 < ?c1") 
+    and f2: "(b + sqrt (b\<^sup>2 + 4 * a)) < 0"
+    using sqrt_ge_absD[of b "b\<^sup>2 + 4 * a"] assms by (force, linarith)
+  hence f3: "exp (t * ?c2 / 2) \<le> exp (t * ?c1 / 2)" (is "exp ?t1 \<le> exp ?t2")
+    unfolding exp_le_cancel_iff 
+    using assms(4) by (case_tac "t=0", simp_all)
+  hence "?c2 * exp ?t2 \<le> ?c2 * exp ?t1"
+    using f1 f2 mult_le_cancel_iff2[of "-?c2" "exp ?t1" "exp ?t2"] by linarith 
+  also have "... < ?c1 * exp ?t1"
+    using f1 by auto
+  also have"... \<le> ?c1 * exp ?t1"
+    using f1 f2 by auto
+  ultimately have "?c2 * exp ?t2 \<le> ?c1 * exp ?t1"
+    using f1 assms(5) by auto
+  hence "(?c2 * exp ?t2) * (k / ?c3) \<le> (?c1 * exp ?t1) * (k / ?c3)"
+    using f0 mult_right_mono by blast
+  thus ?thesis
+    by (auto simp: field_simps)
+qed
+
+dataspace harmonic_osc =
+  constants
+    a :: real
+    b :: real
+  variables 
+    x :: real 
+    y :: real 
+
+context harmonic_osc
+begin
+
+abbreviation mtx_hosc :: "2 sq_mtx" ("A")
+  where "A \<equiv> mtx  
+   ([0, 1] # 
+    [a, b] # [])"
+
+lemma mtx_hosc_nths:
+  "A $$ 1 = (\<chi> i. if i=1 then 0 else 1)"
+  "A $$ 2 = (\<chi> i. if i=1 then a else b)"
+  "A $$ 1 $ 1 = 0" "A $$ 1 $ 2 = 1"
+  "A $$ 2 $ 1 = a" "A $$ 2 $ 2 = b"
+  using exhaust_2
+  by (auto simp: vec_eq_iff)
+
+lemma A_vec_mult_eq: "A *\<^sub>V s = vector [s$2, a * s$1 + b * s$2]"
+  using exhaust_2
+  by (clarsimp simp: vec_eq_iff vector_nth_eq 
+      sq_mtx_vec_mult_eq UNIV_2)
+
+definition "discr \<equiv> sqrt (b\<^sup>2 + 4 * a)"
+
+lemma discr_alt: "discr = sqrt (b\<^sup>2 + a * 4)"
+  by (clarsimp simp: discr_def)
+
+definition  iota1 :: "real" ("\<iota>\<^sub>1")
+  where "\<iota>\<^sub>1 \<equiv> (b - discr)/2"
+
+definition iota2 :: "real" ("\<iota>\<^sub>2")
+  where "\<iota>\<^sub>2 \<equiv> (b + discr)/2"
+
+abbreviation "x_sol t x1 y1 \<equiv> 
+    (1/discr) * x1 * \<iota>\<^sub>2 * exp (t * \<iota>\<^sub>1) - (1/discr) * x1 * \<iota>\<^sub>1 * exp (t * \<iota>\<^sub>2)
+  + (1/discr) * y1 * exp (t * \<iota>\<^sub>2) - (1/discr) * y1 * exp (t * \<iota>\<^sub>1)"
+
+abbreviation "y_sol t x1 y1 \<equiv> 
+    (1/discr) * x1 * a * exp (t * \<iota>\<^sub>2) - (1/discr) * x1 * a * exp (t * \<iota>\<^sub>1)
+  + (1/discr) * y1 * \<iota>\<^sub>2 * exp (t * \<iota>\<^sub>2) - (1/discr) * y1 * \<iota>\<^sub>1 * exp (t * \<iota>\<^sub>1)"
+
+abbreviation "\<Phi> t \<equiv> mtx (
+   [\<iota>\<^sub>2*exp(t*\<iota>\<^sub>1) - \<iota>\<^sub>1*exp(t*\<iota>\<^sub>2),     exp(t*\<iota>\<^sub>2)-exp(t*\<iota>\<^sub>1)]#
+   [a*exp(t*\<iota>\<^sub>2) - a*exp(t*\<iota>\<^sub>1), \<iota>\<^sub>2*exp(t*\<iota>\<^sub>2)-\<iota>\<^sub>1*exp(t*\<iota>\<^sub>1)]#[])"
+
+lemma x_sol_eq: "x_sol t x1 y1 = (((1/discr) *\<^sub>R \<Phi> t) *\<^sub>V (vector [x1,y1])) $ (1::2)"
+  apply (clarsimp simp: sq_mtx_vec_mult_eq UNIV_2)
+  by distribute (simp add: mult.commute diff_divide_distrib)
+
+lemma y_sol_eq: "y_sol t x1 y1 = (((1/discr) *\<^sub>R \<Phi> t) *\<^sub>V (vector [x1,y1])) $ (2::2)"
+  apply (clarsimp simp: sq_mtx_vec_mult_eq UNIV_2)
+  by distribute (simp add: mult.commute mult.left_commute diff_divide_distrib)
+
+abbreviation chB_hosc :: "real \<Rightarrow> real \<Rightarrow> 2 sq_mtx" ("P")
+  where "P a1 a2 \<equiv> mtx
+   ([a1, a2] # 
+    [1, 1] # [])"
+
+lemma inv_mtx_chB_hosc: 
+  "a1 \<noteq> a2 \<Longrightarrow> (P a1 a2)\<^sup>-\<^sup>1 = (1/(a1 - a2)) *\<^sub>R mtx 
+   ([ 1, -a2] # 
+    [-1,  a1] # [])"
+  apply(rule sq_mtx_inv_unique, unfold scaleR_mtx2 times_mtx2)
+  by (simp add: diff_divide_distrib[symmetric] one_mtx2)+
+
+lemma invertible_mtx_chB_hosc: "a1 \<noteq> a2 \<Longrightarrow> mtx_invertible (P a1 a2)"
+  apply(rule mtx_invertibleI[of _ "(P a1 a2)\<^sup>-\<^sup>1"])
+   apply(unfold inv_mtx_chB_hosc scaleR_mtx2 times_mtx2 one_mtx2)
+  by (subst sq_mtx_eq_iff, simp add: vector_def frac_diff_eq1)+
+
+lemma mtx_hosc_diagonalizable:
+  assumes "b\<^sup>2 + a * 4 > 0" and "a \<noteq> 0"
+  shows "A = P (-\<iota>\<^sub>2/a) (-\<iota>\<^sub>1/a) * (\<d>\<i>\<a>\<g> i. if i = 1 then \<iota>\<^sub>1 else \<iota>\<^sub>2) * (P (-\<iota>\<^sub>2/a) (-\<iota>\<^sub>1/a))\<^sup>-\<^sup>1"
+  unfolding assms apply(subst inv_mtx_chB_hosc)
+  using assms apply(simp_all add: diag2_eq[symmetric])
+  apply (simp add: iota1_def discr_def iota2_def)
+  unfolding sq_mtx_times_eq sq_mtx_scaleR_eq UNIV_2 apply(subst sq_mtx_eq_iff)
+  using exhaust_2 assms 
+  by (auto simp: field_simps) 
+    (auto simp: iota1_def iota2_def discr_def field_simps)
+
+lemma mtx_hosc_solution_eq:
+  assumes "b\<^sup>2 + a * 4 > 0" and "a \<noteq> 0"
+  shows "P (-\<iota>\<^sub>2/a) (-\<iota>\<^sub>1/a) * (\<d>\<i>\<a>\<g> i. exp (t * (if i=1 then \<iota>\<^sub>1 else \<iota>\<^sub>2))) * (P (-\<iota>\<^sub>2/a) (-\<iota>\<^sub>1/a))\<^sup>-\<^sup>1 
+  = (1/discr) *\<^sub>R (\<Phi> t)"
+  unfolding assms apply(subst inv_mtx_chB_hosc)
+  using assms apply (simp add: iota1_def discr_def iota2_def)
+  using assms apply(simp_all add: mtx_times_scaleR_commute, subst sq_mtx_eq_iff)
+  unfolding UNIV_2 sq_mtx_times_eq sq_mtx_scaleR_eq sq_mtx_uminus_eq apply(simp_all add: axis_def)
+  by (auto simp: field_simps) 
+    (auto simp: iota1_def iota2_def discr_def field_simps)
+
+lemma local_lipschitz_hosc: 
+  "local_lipschitz UNIV UNIV (loc_subst (x +\<^sub>L y) (\<lambda>t::real. [x \<leadsto> y, y \<leadsto> a * x + b * y]) s)"
+  apply expr_simp
+  by (rule_tac \<DD>="(\<lambda>c. (snd c, a * fst c + b * snd c))" in c1_local_lipschitz)
+    (auto intro!: derivative_eq_intros continuous_intros)
+
+lemma sols_to_Phi: "(x1 * \<iota>\<^sub>2 * exp (t * \<iota>\<^sub>1) / discr - x1 * \<iota>\<^sub>1 * exp (t * \<iota>\<^sub>2) / discr 
+      + y1 * exp (t * \<iota>\<^sub>2) / discr - y1 * exp (t * \<iota>\<^sub>1) / discr,
+        x1 * a * exp (t * \<iota>\<^sub>2) / discr - x1 * a * exp (t * \<iota>\<^sub>1) / discr 
+      + y1 * \<iota>\<^sub>2 * exp (t * \<iota>\<^sub>2) / discr - y1 * \<iota>\<^sub>1 * exp (t * \<iota>\<^sub>1) / discr) = 
+  (((1/discr) *\<^sub>R \<Phi> t) *\<^sub>V (vector [x1,y1]) $ (1::2), 
+  ((1/discr) *\<^sub>R \<Phi> t) *\<^sub>V (vector [x1,y1]) $ (2::2))"
+  apply (clarsimp simp: sq_mtx_vec_mult_eq UNIV_2)
+  apply distribute
+  by (clarsimp simp: add_divide_distrib diff_divide_distrib mult.commute)
+    (simp add: mult.left_commute)
+
+lemma vecf_to_A: "(
+        x1 * a * exp (t * \<iota>\<^sub>2) / discr - x1 * a * exp (t * \<iota>\<^sub>1) / discr 
+      + y1 * \<iota>\<^sub>2 * exp (t * \<iota>\<^sub>2) / discr - y1 * \<iota>\<^sub>1 * exp (t * \<iota>\<^sub>1) / discr,
+   a * (x1 * \<iota>\<^sub>2 * exp (t * \<iota>\<^sub>1) / discr - x1 * \<iota>\<^sub>1 * exp (t * \<iota>\<^sub>2) / discr 
+      + y1 * exp (t * \<iota>\<^sub>2) / discr - y1 * exp (t * \<iota>\<^sub>1) / discr) 
+ + b * (x1 * a * exp (t * \<iota>\<^sub>2) / discr - x1 * a * exp (t * \<iota>\<^sub>1) / discr 
+      + y1 * \<iota>\<^sub>2 * exp (t * \<iota>\<^sub>2) / discr - y1 * \<iota>\<^sub>1 * exp (t * \<iota>\<^sub>1) / discr)
+    ) = 
+    (
+      (A *\<^sub>V (((1/discr) *\<^sub>R \<Phi> t) *\<^sub>V (vector [x1,y1]))) $ (1::2), 
+      (A *\<^sub>V (((1/discr) *\<^sub>R \<Phi> t) *\<^sub>V (vector [x1,y1]))) $ (2::2)
+    )"
+  apply (clarsimp simp: sq_mtx_vec_mult_eq UNIV_2)
+  apply distribute
+  apply (clarsimp simp: add_divide_distrib diff_divide_distrib mult.commute)
+  apply (simp add: mult.left_commute)
+  apply distribute
+  by (clarsimp simp: add_divide_distrib diff_divide_distrib mult.commute)
+
+lemma local_flow_mtx_hosc:
+  assumes "b\<^sup>2 + a * 4 > 0" and "a \<noteq> 0"
+  shows "local_flow ((*\<^sub>V) A) UNIV UNIV (\<lambda>t. (*\<^sub>V) ((1/discr) *\<^sub>R \<Phi> t))"
+  unfolding assms using local_flow_sq_mtx_linear[of "A"] assms
+  apply(subst (asm) exp_scaleR_diagonal2[OF invertible_mtx_chB_hosc mtx_hosc_diagonalizable])
+     apply(simp add: iota1_def iota2_def discr_def, simp, simp)
+  by (subst (asm) mtx_hosc_solution_eq) simp_all
+
+lemma has_vderiv_Phi_A: "0 < b\<^sup>2 + a * 4 \<Longrightarrow> a \<noteq> 0 
+  \<Longrightarrow> ((\<lambda>t. ((1 / discr) *\<^sub>R \<Phi> t) *\<^sub>V s) has_vderiv_on (\<lambda>t. A *\<^sub>V (((1 / discr) *\<^sub>R \<Phi> t) *\<^sub>V s))) {0--t}"
+  using conjunct1[OF conjunct2[OF local_flow_mtx_hosc[unfolded local_flow_def local_flow_axioms_def]]] 
+  by clarsimp
+
+lemma local_flow_hosc: "a \<noteq> 0 \<Longrightarrow> b\<^sup>2 + 4 * a > 0
+  \<Longrightarrow> local_flow_on [x \<leadsto> y, y \<leadsto> a * x + b * y] (x +\<^sub>L y) UNIV UNIV
+  (\<lambda>t. [x \<leadsto> x_sol t x y, y \<leadsto> y_sol t x y])"
+  unfolding local_flow_on_def 
+  unfolding local_flow_def local_flow_axioms_def apply safe
+  using local_lipschitz_hosc
+     apply (unfold_locales; clarsimp?)
+    apply (expr_simp add: x_sol_eq y_sol_eq)
+    apply (subst sols_to_Phi)
+    apply (subst vecf_to_A)
+    prefer 3 subgoal by expr_simp
+   prefer 2 subgoal 
+    apply (expr_simp add: iota1_def iota2_def)
+    by distribute (clarsimp simp: add_divide_distrib diff_divide_distrib discr_def)
+  apply (rename_tac x1 y1)
+  apply (rule poly_derivatives)
+    prefer 3 apply force
+  apply (rule iffD1[OF has_vderiv_on_component, rule_format]) (* name this lemma *)
+   apply (rule has_vderiv_Phi_A, simp, simp)
+  apply (rule iffD1[OF has_vderiv_on_component, rule_format]) (* name this lemma *)
+  by (rule has_vderiv_Phi_A, simp, simp)
+
+
+lemma "a < 0 \<Longrightarrow> b \<le> 0 \<Longrightarrow> b\<^sup>2 + 4 * a > 0 \<Longrightarrow>
+  \<^bold>{x=0\<^bold>} 
+  LOOP (
+    (x ::= ?);(y ::= 0); \<questiondown>x>0?;
+    {x` = y, y` = a * x + b * y}
+  ) INV (x\<ge>0)
+  \<^bold>{x\<ge>0\<^bold>}"
+  apply (rule hoare_loopI)
+    prefer 3 apply expr_simp
+   prefer 2 apply expr_simp
+  apply (clarsimp simp add: wp fbox_g_dL_easiest[OF local_flow_hosc])
+  apply expr_simp
+  apply (clarsimp simp: iota1_def iota2_def discr_def)
+  using overdamped_door_arith[of b a] by force
+
 
 end
 
